thinking...

Decompose_Update.thy
@@ -30,58 +30,11 @@ type_synonym ('y, 'b) store = "'y index \<Rightarrow> 'b list"
 
 subsection \<open>Utility functions\<close>
 
-(* obtain the first string (of alphabet) before any variable *)
-fun first_string :: "('x + 'b) list \<Rightarrow> 'b list" where
-  "first_string [] = []" |
-  "first_string (Inl x#xs) = []" |
-  "first_string (Inr b#xs) = b # first_string xs"
-
-(* skip input characters until a variable specified occurs *)
-fun skip_until_var :: "('y + 'b) list \<Rightarrow> ('y + 'b) list" where
-  "skip_until_var [] = []" |
-  "skip_until_var (Inl x#xs) = xs" |
-  "skip_until_var (Inr b#xs) = skip_until_var xs"
-
-(* skip input characters until a variable specified occurs *)
-fun skip_until :: "'y index \<Rightarrow> ('y index + 'b) list \<Rightarrow> ('y index + 'b) list" where
-  "skip_until y' [] = []" |
-  "skip_until (x, y, k) (Inl (x0, y0, k0)#xs) = 
-    (if k = k0 then xs else skip_until (x, y, k) xs)" |
-  "skip_until y' (Inr b#xs) = skip_until y' xs"
-
-fun nth_string :: "nat \<Rightarrow> ('y + 'b) list \<Rightarrow> 'b list" where
-  "nth_string 0 xs = first_string xs" |
-  poyo: "nth_string (Suc n) xs = nth_string n (skip_until_var xs)"
-
 
 fun extract_variables :: "('x + 'b) list \<Rightarrow> 'x list" where
   "extract_variables [] = []" |
   "extract_variables (Inl x#xs) = x # extract_variables xs" |
   "extract_variables (Inr a#xs) = extract_variables xs"
-
-fun give_indices_rec :: "nat \<Rightarrow> 'x \<Rightarrow> ('x + 'b) list \<Rightarrow> ('x index + 'b) list" where
-  "give_indices_rec cnt x [] = []" |
-  "give_indices_rec cnt x (Inl y#ys) = Inl (x, y, cnt) # give_indices_rec (Suc cnt) x ys" |
-  "give_indices_rec cnt x (Inr b#ys) = Inr b # give_indices_rec cnt x ys"
-
-fun give_indices :: "'x \<Rightarrow> ('x + 'b) list \<Rightarrow> ('x index + 'b) list" where
-  "give_indices x ys = give_indices_rec 0 x ys"
-
-subsection \<open>Resolve\<close>
-
-(*
-fun scan_pair2 where
-  "scan_pair2 x [] = [(x, [])]" |
-  "scan_pair2 x (Inl y#u) = (x, []) # scan_pair2 y u" |
-  "scan_pair2 x (Inr a#u) = (case scan_pair2 x u of
-     ((y, as)#pairs) \<Rightarrow> (y, a#as) # pairs)"
-
-fun scan02 where
-  "scan02 [] = ([], [])" |
-  "scan02 (Inl x#u) = ([], scan_pair2 x u)" |
-  "scan02 (Inr a#u) = (let (as, pair) = scan02 u in (a # as, pair))"
-  
-*)
 
 fun scan_pair where
   "scan_pair x as [] = [(x, as)]" |
@@ -103,19 +56,18 @@ fun flat_rec where
 fun flat where
   "flat (b0, xas) = map Inr b0 @ flat_rec xas"
 
-fun replace_rec where
-  "replace_rec y n [] = []" |
-  "replace_rec y n ((x, _)#xs) = Inl x # Inr (y, n) # replace_rec y (Suc n) xs"
+fun padding_rec :: "nat \<Rightarrow> 'x \<Rightarrow> ('x \<times> 'b list) list \<Rightarrow> ('x + 'x index) list" where
+  "padding_rec n y [] = []" |
+  "padding_rec n y ((x, _)#xs) = Inl x # Inr (y, n) # padding_rec (Suc n) y xs"
 
-fun replace where
-  "replace y (a0, xs) = Inr (y, 0) # replace_rec y 1 xs"
+fun padding where
+  "padding y (a0, xs) = Inr (y, 0) # padding_rec 1 y xs"
+
 
 fun ith_string where
   "ith_string [] k = []" |
   "ith_string ((x,as)#xas) 0 = as" |
   "ith_string (_#xas) (Suc k) = ith_string xas k"
-
-
 
 lemma flat_rec_scan_pair: "flat_rec (scan_pair x as u) = Inl x # map Inr as @ u"
   by (induct u arbitrary: x as rule: xa_induct, simp_all)
@@ -127,78 +79,74 @@ lemma "flat (scan u) = u"
   by (induct u rule: xa_induct, simp_all add: flat_rec_scan_pair flat_scan0)
 
 
+subsection \<open>Resolve\<close>
+
+(*
+fun scan_pair2 where
+  "scan_pair2 x [] = [(x, [])]" |
+  "scan_pair2 x (Inl y#u) = (x, []) # scan_pair2 y u" |
+  "scan_pair2 x (Inr a#u) = (case scan_pair2 x u of
+     ((y, as)#pairs) \<Rightarrow> (y, a#as) # pairs)"
+
+fun scan02 where
+  "scan02 [] = ([], [])" |
+  "scan02 (Inl x#u) = ([], scan_pair2 x u)" |
+  "scan02 (Inr a#u) = (let (as, pair) = scan02 u in (a # as, pair))"
+  
+*)
+
 definition resolve_shuffle :: "('y, 'b) update \<Rightarrow> 'y shuffle" where
   "resolve_shuffle \<theta> y = extract_variables (\<theta> y)"
 
-fun resolve_store :: "('y, 'b) update \<Rightarrow> ('y, 'b) store" where
-  "resolve_store \<theta> (x, 0) = fst (scan (\<theta> x))" |
-  "resolve_store \<theta> (x, k) = ith_string (snd (scan (\<theta> x))) k"
+definition resolve_store :: "('y, 'b) update \<Rightarrow> ('y, 'b) store" where
+  "resolve_store \<theta> y = (case y of
+     (x, 0) \<Rightarrow> fst (scan (\<theta> x)) |
+     (x, Suc k) \<Rightarrow> ith_string (snd (scan (\<theta> x))) k)"
+
+fun resolve :: "('y, 'b) update \<Rightarrow> 'y shuffle \<times> ('y, 'b) store" where
+  "resolve \<theta> = (resolve_shuffle \<theta>, resolve_store \<theta>)"
 
 
 subsection \<open>Synthesize\<close>
 
-definition synthesize_shuffle :: "'y shuffle \<Rightarrow> ('y, 'y index, 'b) update'" where
-  "synthesize_shuffle s y = give_indices y (map Inl (s y))"
+definition synthesize_shuffle :: "'y shuffle \<Rightarrow> ('y, 'y + 'y index, 'b) update'" where
+  "synthesize_shuffle s y = map Inl (padding y (scan (map Inl (s y) :: ('y + 'y) list)))"
 
-definition synthesize_prepend :: "('y, 'b) prepend \<Rightarrow> ('y, 'y, 'b) update'" where
-  "synthesize_prepend a y = map Inr (a y) @ [Inl y]"
+definition synthesize_store :: "('y, 'b) store \<Rightarrow> ('y + 'y index, 'y, 'b) update'" where
+  "synthesize_store a yi = (case yi of
+     (Inl y) \<Rightarrow> [Inl y] | 
+     (Inr i) \<Rightarrow> map Inr (a i))"
 
-definition synthesize_append :: "('y, 'b) append \<Rightarrow> ('y index, 'y, 'b) update'" where
-  "synthesize_append a = (\<lambda>(x, y, k). Inl y # map Inr (a (x, y, k)))"
-
-
-
-
-definition synthesize :: "'y shuffle \<times> ('y, 'b) store \<Rightarrow> ('y, 'b) update" where
-  "synthesize sap = (case sap of (s, a, p) \<Rightarrow>
-     synthesize_append a \<bullet> synthesize_shuffle s \<bullet> synthesize_prepend p)"
-
-fun lookup_store :: "('y, 'b) store \<Rightarrow> 'y location \<Rightarrow> 'b list" where
-  "lookup_store (a, p) (Inl i) = a i" |
-  "lookup_store (a, p) (Inr y) = p y"
+fun synthesize :: "'y shuffle \<times> ('y, 'b) store \<Rightarrow> ('y, 'b) update" where
+  "synthesize (s, a) = synthesize_store a \<bullet> synthesize_shuffle s"
 
 
 subsection \<open>Properties of Decomposition\<close>
 
-lemma give_indices_rec_Inr: "give_indices_rec k x (map Inr as @ xs) = map Inr as @ give_indices_rec k x xs"
-  by (induct as, simp_all)
-
-lemma hat_alpha_give_indices_left: "hat_alpha t (give_indices_rec k x u) = give_indices_rec k x (hat_alpha t u)"
-proof (induct u arbitrary: k rule: xa_induct)
-  case Nil
-  then show ?case by simp
-next
-  case (Var x xs)
-  then show ?case by simp
-next
-  case (Alpha a xs)
-  then show ?case by (simp add: give_indices_rec_Inr)
+lemma ext_sum:
+  assumes "\<And>l. f (Inl l) = g (Inl l)"
+  assumes "\<And>r. f (Inr r) = g (Inr r)"
+  shows "f = g"
+proof
+  fix x
+  show "f x = g x" using assms by (cases x, simp_all)
 qed
 
-lemma map_alpha_synthesize_append: "t \<star> synthesize_append a = synthesize_append (concat o map t o a)"
-  by (auto simp add: synthesize_append_def map_alpha_def hat_alpha_right_map)
-
 lemma map_alpha_synthesize_shuffle: "t \<star> synthesize_shuffle s = synthesize_shuffle s"
-  by (rule ext, auto simp add: synthesize_shuffle_def map_alpha_def hat_alpha_right_map 
-      hat_alpha_give_indices_left hat_alpha_left_ignore)
+  by (auto simp add: map_alpha_def hat_alpha_left_ignore synthesize_shuffle_def)
 
-lemma map_alpha_synthesize_prepend: "t \<star> synthesize_prepend p = synthesize_prepend (concat o map t o p)"
-  by (auto simp add: synthesize_prepend_def map_alpha_def hat_alpha_right_map)
+lemma map_alpha_synthesize_store: "t \<star> synthesize_store p = synthesize_store (concat o map t o p)"
+  by (rule ext_sum, simp_all add: map_alpha_def Update.hat_alpha_right_map synthesize_store_def)
 
-lemma map_alpha_synthesize: "t \<star> synthesize (s, a, p) = synthesize (s, concat o map t o a, concat o map t o p)"
-  by (simp add: synthesize_def map_alpha_distrib
-      map_alpha_synthesize_shuffle map_alpha_synthesize_append map_alpha_synthesize_prepend)
-
-lemma concat_map_resolve_append: "(concat o map t) (resolve_append \<theta> y) = resolve_append (t \<star> \<theta>) y"
-  apply (simp add: resolve_append_def)
+lemma map_alpha_synthesize: "t \<star> synthesize (s, a) = synthesize (s, concat o map t o a)"
+  by (auto simp add: map_alpha_distrib map_alpha_synthesize_shuffle map_alpha_synthesize_store)
 
 lemma resolve_idU_idS: "resolve_shuffle idU = idS"
-  by (rule ext, simp add: idU_def idS_def resolve_shuffle_def)
+  by (auto simp add: idU_def idS_def resolve_shuffle_def)
 
 theorem resolve_inverse: "synthesize (resolve m) x = m x"
+  apply (simp add: comp_def)
   oops
-
-
 
 
 
@@ -218,27 +166,29 @@ theorem resolve_inverse: "synthesize (resolve m) x = m x"
 
 subsection \<open>Example\<close>
 
-fun poyo :: "(int, char) update" where
-  "poyo z = (if z = 0 then [Inr (CHR ''P''), Inl 0, Inr (CHR ''Q''), Inl 0, Inr (CHR ''R'')]
+definition poyo :: "(int, char) update" where
+  "poyo = (%z. if z = 0 then [Inr (CHR ''P''), Inl 0, Inr (CHR ''Q''), Inl 0, Inr (CHR ''R'')]
         else if z = 1 then [Inr (CHR ''A''), Inl 0, Inr (CHR ''B''), Inl 1, Inr (CHR ''C'')]
         else [])"
 
-lemma "resolve_prepend poyo 0 = ''P''" by (simp add: resolve_prepend_def)
-lemma "resolve_prepend poyo 1 = ''A''" by (simp add: resolve_prepend_def)
+declare poyo_def [simp]
 
-lemma "resolve_append poyo (0, 0, 0) = ''Q''" by (simp add: resolve_append_def)
-lemma "resolve_append poyo (0, 0, 1) = ''R''" by (simp add: resolve_append_def)
-lemma "resolve_append poyo (1, 0, 0) = ''B''" by (simp add: resolve_append_def)
-lemma "resolve_append poyo (1, 1, 1) = ''C''" by (simp add: resolve_append_def)
+value "poyo 1"
+value "resolve_store poyo (0, 2)"
+value "resolve_store poyo (0, 3)"
+
+lemma "resolve_shuffle poyo 0 = [0, 0]" by simp
+lemma "resolve_shuffle poyo 1 = [0, 1]" by simp
+
+lemma "resolve_store poyo (0, 0) = ''P''" by simp
+lemma "resolve_store poyo (0, 1) = ''Q''" by simp
+lemma "resolve_store poyo (0, 2) = ''R''" oops
+lemma "resolve_store poyo (1, 0) = ''A''" by simp
+lemma "resolve_store poyo (1, 1) = ''B''" by simp
 
 
-lemma "resolve_shuffle poyo 0 = [0, 0]" by (simp add: resolve_shuffle_def)
-
-
-(*
 lemma "synthesize (resolve poyo) x = poyo x"
-  by (simp add: synthesize_def resolve_def comp_def)
+  by (simp add: comp_def)
 
-*)
 
 end
